Done `programming-language-foundations/StlcProp.v`

programming-language-foundations/StlcProp.v
@@ -145,7 +145,21 @@ Theorem progress' : forall t T,
 Proof.
   intros t.
   induction t; intros T Ht; auto.
-  (* FILL IN HERE *) Admitted.
+  - inversion Ht; subst. discriminate H1.
+  - inversion Ht; subst. inversion Ht; subst. right.
+    apply IHt1 in H2. apply IHt2 in H4.
+    destruct H2 as [Ht1|[t1' Ht1]].
+    + destruct H4 as [Ht2|[t2' Ht2]].
+      * eapply canonical_forms_fun in Ht1; [|apply H3].
+        destruct Ht1 as [x [t0 H1]]; subst.
+        exists (<{ [x:=t2] t0 }>). eauto.
+      * exists (<{ t1 t2' }>). eauto.
+    + exists (<{ t1' t2 }>). eauto.
+  - inversion Ht; subst. inversion Ht; subst. right. apply IHt1 in H3.
+    destruct H3 as [Ht1|[t1' Ht1]].
+    + destruct (canonical_forms_bool t1); subst; eauto.
+    + exists (<{ if t1' then t2 else t3 }>). eauto.
+Qed.
 (** [] *)
 
 (* ################################################################# *)
@@ -332,7 +346,14 @@ Proof.
   remember (x |-> U; Gamma) as Gamma'.
   generalize dependent Gamma.
   induction Ht; intros Gamma' G; simpl; eauto.
- (* FILL IN HERE *) Admitted.
+  - rename x0 into y. destruct (eqb_stringP x y); subst.
+    + rewrite update_eq in H. injection H as H; subst.
+      apply weakening_empty. assumption.
+    + rewrite update_neq in H; [| assumption]. apply T_Var. assumption.
+  - rename x0 into y. destruct (eqb_stringP x y); subst; apply T_Abs.
+    + rewrite update_shadow in Ht. assumption.
+    + apply IHHt. apply update_permute. assumption.
+Qed.
 (** [] *)
 
 (* ================================================================= *)
@@ -418,7 +439,8 @@ Qed.
     You can state your counterexample informally in words, with a brief
     explanation. *)
 
-(* FILL IN HERE *)
+(* [if t1 then t2 else t3], where [t1] can be reduced to [true] or [false],
+   [t2] and [t3] can differ in types, so the whole term does not have a type. *)
 
 (* Do not modify the following line: *)
 Definition manual_grade_for_subject_expansion_stlc : option (nat*string) := None.
@@ -443,7 +465,10 @@ Proof.
   intros t t' T Hhas_type Hmulti. unfold stuck.
   intros [Hnf Hnot_val]. unfold normal_form in Hnf.
   induction Hmulti.
-  (* FILL IN HERE *) Admitted.
+  - apply progress in Hhas_type. destruct Hhas_type as [Hval|Hnot_nf]; contradiction.
+  - eapply preservation in Hhas_type; [|apply H].
+    apply IHHmulti in Hhas_type; assumption.
+Qed.
 (** [] *)
 
 (* ################################################################# *)
@@ -459,7 +484,16 @@ Theorem unique_types : forall Gamma e T T',
   Gamma |- e \in T' ->
   T = T'.
 Proof.
-  (* FILL IN HERE *) Admitted.
+  intros Gamma e. 
+  generalize dependent Gamma.
+  induction e; intros; inversion H; subst; inversion H0; subst; auto.
+  - rewrite H3 in H4. injection H4 as H4. auto.
+  - eapply IHe1 in H4; [|apply H5].
+    eapply IHe2 in H6; [|apply H8].
+    subst. injection H4 as H4. auto.
+  - eapply IHe in H6; [| apply H7]. subst. reflexivity.
+  - eapply IHe2 in H7; [| apply H10]. symmetry. assumption.
+Qed.
 (** [] *)
 
 (* ################################################################# *)
@@ -534,7 +568,34 @@ Definition closed (t:tm) :=
     understanding it is crucial to understanding substitution and its
     properties, which are really the crux of the lambda-calculus. *)
 
-(* FILL IN HERE *)
+(* 
+             ---------------------------- (afi_var)
+                x apperas_free_in <{x}>
+
+                x apperas_free_in <t1>
+             ---------------------------- (afi_app1)
+                x apperas_free_in <{t1 t2}>
+
+                x apperas_free_in <t2>
+             ---------------------------- (afi_app2)
+                x apperas_free_in <{t1 t2}>
+
+                x apperas_free_in <t1>     y <> x
+             --------------------------------------- (afi_abs)
+                x apperas_free_in <{\y:T1, t1}>
+
+                x apperas_free_in <t1>
+             ------------------------------------------------ (afi_if1)
+                x apperas_free_in <{if t1 then t2 else t3}>
+
+                x apperas_free_in <t2>
+             ------------------------------------------------ (afi_if2)
+                x apperas_free_in <{if t1 then t2 else t3}>
+
+                x apperas_free_in <t3>
+             ------------------------------------------------ (afi_if3)
+                x apperas_free_in <{if t1 then t2 else t3}>
+*)
 
 (* Do not modify the following line: *)
 Definition manual_grade_for_afi : option (nat*string) := None.
@@ -587,7 +648,12 @@ Proof.
   generalize dependent T.
   induction H;
          intros; try solve [inversion H0; eauto].
-  (* FILL IN HERE *) Admitted.
+  inversion H1; subst.
+  apply IHappears_free_in in H7.
+  destruct H7 as [T' H2].
+  rewrite update_neq in H2; [|assumption].
+  exists T'. assumption.
+Qed.
 (** [] *)
 
 (** From the [free_in_context] lemma, it immediately follows that any
@@ -599,7 +665,11 @@ Corollary typable_empty__closed : forall t T,
     empty |- t \in T  ->
     closed t.
 Proof.
-  (* FILL IN HERE *) Admitted.
+  intros t T H x Hc.
+  eapply free_in_context in Hc; [|eassumption].
+  destruct Hc as [T' Hc].
+  inversion Hc.
+Qed.
 (** [] *)
 
 (** Finally, we establish _context_invariance_.  It is useful in cases
@@ -661,7 +731,14 @@ Proof.
   intros.
   generalize dependent Gamma'.
   induction H; intros; auto.
-  (* FILL IN HERE *) Admitted.
+  - constructor. rewrite <- H. specialize H0 with x0. symmetry. apply H0. constructor.
+  - constructor. apply IHhas_type. intros y Hy. destruct (eqb_stringP x0 y); subst.
+    + repeat rewrite update_eq. auto.
+    + eapply afi_abs in Hy; [|eassumption].
+      repeat rewrite update_neq; try apply H0; eassumption.
+  - econstructor; [apply IHhas_type1 | apply IHhas_type2];
+    intros x Hx; apply H1; [ apply afi_app1 | apply afi_app2 ]; assumption.
+Qed.
 (** [] *)
 
 (** The context invariance lemma can actually be used in place of the
@@ -678,7 +755,16 @@ Proof.
     Coq theorems).
     You can write [Admitted] for the proofs. *)
 
-(* FILL IN HERE *)
+Theorem progress'' : forall x T,
+  empty |- x \in T ->
+  value x \/ (exists x', x --> x').
+Admitted.
+
+Theorem preservation' : forall x y T,
+  empty |- x \in T ->
+  x --> y ->
+  empty |- y \in T.
+Admitted.
 
 (* Do not modify the following line: *)
 Definition manual_grade_for_progress_preservation_statement : option (nat*string) := None.
@@ -702,11 +788,13 @@ and the following typing rule:
     false, give a counterexample.
 
       - Determinism of [step]
-(* FILL IN HERE *)
+        Becomes false. Let [t] = [(\x: Bool x) true]. We have
+        both [t --> true] and [t --> zap].
       - Progress
-(* FILL IN HERE *)
+        Becomes false. Let [t] = [zap], we have [empty |- zap \in T] but
+        neither [value t] nor [exists t', zap --> t'].
       - Preservation
-(* FILL IN HERE *)
+        Remains true.
 *)
 
 (* Do not modify the following line: *)
@@ -730,11 +818,14 @@ Definition manual_grade_for_stlc_variation1 : option (nat*string) := None.
     false, give a counterexample.
 
       - Determinism of [step]
-(* FILL IN HERE *)
+        Becomes false. [(\x:Bool, x) true] --> [true] by [ST_AppAbs],
+        but [(\x:Bool, x) true] --> [foo true] by [ST_App1] & [ST_Foo1].
       - Progress
-(* FILL IN HERE *)
+        Remains true.
       - Preservation
-(* FILL IN HERE *)
+        Becomes false. [empty |- (\x:Bool, x) true \in Bool] ->
+        [(\x:Bool, x) true --> foo true] ->
+        ~[empty |- foo true \in Bool].
 *)
 
 (* Do not modify the following line: *)
@@ -750,11 +841,12 @@ Definition manual_grade_for_stlc_variation2 : option (nat*string) := None.
     false, give a counterexample.
 
       - Determinism of [step]
-(* FILL IN HERE *)
+        Remains true.
       - Progress
-(* FILL IN HERE *)
+        Becomes false. Neight [((\x:Bool->Bool->Bool, true) true) true] is
+        a [value] nor it can step.
       - Preservation
-(* FILL IN HERE *)
+        Remains true.
 *)
 
 (* Do not modify the following line: *)
@@ -775,11 +867,12 @@ Definition manual_grade_for_stlc_variation3 : option (nat*string) := None.
     false, give a counterexample.
 
       - Determinism of [step]
-(* FILL IN HERE *)
+        Becomes false. [if true then false else true] --> [true] by [ST_FunnyIfTrue]
+        byt [if true then false else true] --> [false] by [ST_IfTrue].
       - Progress
-(* FILL IN HERE *)
+        Remains true.
       - Preservation
-(* FILL IN HERE *)
+        Remains true.
 *)
 (** [] *)
 
@@ -799,11 +892,21 @@ Definition manual_grade_for_stlc_variation3 : option (nat*string) := None.
     false, give a counterexample.
 
       - Determinism of [step]
-(* FILL IN HERE *)
+        Remains true.
       - Progress
-(* FILL IN HERE *)
+        Remains true.
       - Preservation
-(* FILL IN HERE *)
+        Becomes false. Let [Gamma |- t1 \in Bool->Bool->Bool],
+        [Gamma |- t2 \in Bool],
+        then we have [Gamma |- t1 t2 \in Bool] by [T_FunnyApp],
+        and [Gamma |- t1 t2 \in Bool->Bool] by [T_App].
+        However, since 
+        + [t1 t2] --> [\y:Bool->Bool, [x := t2] t1'] by [ST_AppAbs],
+           where t1 = [\y:Bool->Bool, t1'],
+        + or [t1 t2] --> [t1' t2] by [ST_App1], where [t1 --> t1'],
+        + or [t1 t2] --> [t1 t2'] by [ST_App2], where [t2 --> t2'],
+        We can conclude that [Gamma |- t' \in Bool->Bool] from the 
+        above 3 cases, which breaks the [preservation] theorem.
 *)
 (** [] *)
 
@@ -823,11 +926,11 @@ Definition manual_grade_for_stlc_variation3 : option (nat*string) := None.
     false, give a counterexample.
 
       - Determinism of [step]
-(* FILL IN HERE *)
+        Remains true.
       - Progress
-(* FILL IN HERE *)
+        Remains true.
       - Preservation
-(* FILL IN HERE *)
+        Becomes false. The same as [T_FunnyApp].
 *)
 (** [] *)
 
@@ -845,11 +948,12 @@ Definition manual_grade_for_stlc_variation3 : option (nat*string) := None.
     false, give a counterexample.
 
       - Determinism of [step]
-(* FILL IN HERE *)
+        Remains true.
       - Progress
-(* FILL IN HERE *)
+        Remains true.
       - Preservation
-(* FILL IN HERE *)
+        Remains true. This `[T_FunnyAbs] only affects the [value]s
+        (that cannot step) of the lambda calculus.
 *)
 (** [] *)
 
@@ -952,7 +1056,506 @@ Coercion tm_const : nat >-> tm.
         STLC to deal with the new syntactic forms. Make sure Coq
         accepts the whole file. *)
 
-(* FILL IN HERE *)
+
+Reserved Notation "'[' x ':=' s ']' t" (in custom stlc at level 20, x constr).
+
+Fixpoint subst (x : string) (s : tm) (t : tm) : tm :=
+  match t with
+  | tm_var y =>
+      if eqb_string x y then s else t
+  | <{\y:T, t1}> =>
+      if eqb_string x y then t else <{\y:T, [x:=s] t1}>
+  | <{t1 t2}> =>
+      <{([x:=s] t1) ([x:=s] t2)}>
+  | tm_const n  =>
+      tm_const n
+  | <{succ t}> =>
+      <{succ [x:=s] t}>
+  | <{pred t}> =>
+      <{pred [x:=s] t}>
+  | <{t1 * t2}> =>
+      <{([x:=s] t1) * ([x:=s] t2)}>
+  | <{if0 t1 then t2 else t3}> =>
+      <{if0 ([x:=s] t1) then ([x:=s] t2) else ([x:=s] t3)}>
+  end
+
+where "'[' x ':=' s ']' t" := (subst x s t) (in custom stlc).
+
+Inductive value : tm -> Prop :=
+  | v_abs : forall x T2 t1,
+      value <{\x:T2, t1}>
+  | v_const : forall n,
+      value (tm_const n).
+
+Hint Constructors value : core.
+
+Reserved Notation "t '-->' t'" (at level 40).
+
+Inductive step : tm -> tm -> Prop :=
+  | ST_AppAbs : forall x T2 t1 v2,
+         value v2 ->
+         <{(\x:T2, t1) v2}> --> <{ [x:=v2]t1 }>
+  | ST_App1 : forall t1 t1' t2,
+         t1 --> t1' ->
+         <{t1 t2}> --> <{t1' t2}>
+  | ST_App2 : forall v1 t2 t2',
+         value v1 ->
+         t2 --> t2' ->
+         <{v1 t2}> --> <{v1  t2'}>
+  | ST_SuccNat : forall n : nat,
+      <{succ n}> --> tm_const (S n)
+  | ST_Succ : forall t t',
+      t --> t' ->
+      <{succ t}> --> <{succ t'}>
+  | ST_PredNat : forall n : nat,
+      <{pred n}> --> tm_const (pred n)
+  | ST_PredSucc : forall t,
+      value t ->
+      <{pred (succ t)}> --> <{t}>
+  | ST_Pred : forall t t',
+      t --> t' ->
+      <{pred t}> --> <{pred t'}>
+  | ST_Mult1 : forall t1 t1' t2,
+      t1 --> t1' ->
+      <{t1 * t2}> --> <{t1' * t2}>
+  | ST_Mult2 : forall t1 t2 t2',
+      value t1 ->
+      t2 --> t2' ->
+      <{t1 * t2}> --> <{t1 * t2'}>
+  | ST_MultNat : forall n1 n2 : nat,
+      <{n1 * n2}> --> tm_const (n1 * n2)
+  | ST_If0Zero : forall t1 t2,
+      <{if0 0 then t1 else t2}> --> t1
+  | ST_If0Succ : forall (n : nat) t1 t2,
+      tm_if0 (S n) t1 t2 --> t2
+  | ST_If0 : forall t1 t1' t2 t3,
+      t1 --> t1' ->
+      <{if0 t1 then t2 else t3}> --> <{if0 t1' then t2 else t3}>
+
+where "t '-->' t'" := (step t t').
+
+Hint Constructors step : core.
+
+Notation multistep := (multi step).
+Notation "t1 '-->*' t2" := (multistep t1 t2) (at level 40).
+
+Definition context := partial_map ty.
+
+Reserved Notation "Gamma '|-' t '\in' T"
+            (at level 101,
+             t custom stlc, T custom stlc at level 0).
+
+Inductive has_type : context -> tm -> ty -> Prop :=
+  | T_Var : forall Gamma x T1,
+      Gamma x = Some T1 ->
+      Gamma |- x \in T1
+  | T_Abs : forall Gamma x T1 T2 t1,
+      x |-> T2 ; Gamma |- t1 \in T1 ->
+      Gamma |- \x:T2, t1 \in (T2 -> T1)
+  | T_App : forall T1 T2 Gamma t1 t2,
+      Gamma |- t1 \in (T2 -> T1) ->
+      Gamma |- t2 \in T2 ->
+      Gamma |- t1 t2 \in T1
+  | T_Const : forall Gamma (n : nat),
+       Gamma |- n \in Nat
+  | T_Succ : forall Gamma t,
+       Gamma |- t \in Nat ->
+       Gamma |- succ t \in Nat
+  | T_Pred : forall Gamma t,
+       Gamma |- t \in Nat ->
+       Gamma |- pred t \in Nat
+  | T_Mult : forall Gamma t1 t2,
+       Gamma |- t1 \in Nat ->
+       Gamma |- t2 \in Nat ->
+       Gamma |- t1 * t2 \in Nat
+  | T_If0 : forall t1 t2 t3 T1 Gamma,
+       Gamma |- t1 \in Nat ->
+       Gamma |- t2 \in T1 ->
+       Gamma |- t3 \in T1 ->
+       Gamma |- if0 t1 then t2 else t3 \in T1
+
+where "Gamma '|-' t '\in' T" := (has_type Gamma t T).
+
+Hint Constructors has_type : core.
+
+Inductive appears_free_in (x : string) : tm -> Prop :=
+  | afi_var : appears_free_in x <{x}>
+  | afi_app1 : forall t1 t2,
+      appears_free_in x t1 ->
+      appears_free_in x <{t1 t2}>
+  | afi_app2 : forall t1 t2,
+      appears_free_in x t2 ->
+      appears_free_in x <{t1 t2}>
+  | afi_abs : forall y T1 t1,
+      y <> x  ->
+      appears_free_in x t1 ->
+      appears_free_in x <{\y:T1, t1}>
+  | afi_succ : forall t1,
+      appears_free_in x t1 ->
+      appears_free_in x <{succ t1}>
+  | afi_pred : forall t1,
+      appears_free_in x t1 ->
+      appears_free_in x <{pred t1}>
+  | afi_multi1 : forall t1 t2,
+      appears_free_in x t1 ->
+      appears_free_in x <{t1 * t2}>
+  | afi_multi2 : forall t1 t2,
+      appears_free_in x t2 ->
+      appears_free_in x <{t1 * t2}>
+  | afi_if01 : forall t1 t2 t3,
+      appears_free_in x t1 ->
+      appears_free_in x <{if0 t1 then t2 else t3}>
+  | afi_if02 : forall t1 t2 t3,
+      appears_free_in x t2 ->
+      appears_free_in x <{if0 t1 then t2 else t3}>
+  | afi_if03 : forall t1 t2 t3,
+      appears_free_in x t3 ->
+      appears_free_in x <{if0 t1 then t2 else t3}>.
+
+Hint Constructors appears_free_in : core.
+
+Lemma weakening : forall Gamma Gamma' t T,
+     inclusion Gamma Gamma' ->
+     Gamma  |- t \in T  ->
+     Gamma' |- t \in T.
+Proof.
+  intros Gamma Gamma' t T H Ht.
+  generalize dependent Gamma'.
+  induction Ht; eauto using inclusion_update.
+Qed.
+
+Lemma weakening_empty : forall Gamma t T,
+     empty |- t \in T  ->
+     Gamma |- t \in T.
+Proof.
+  intros Gamma t T.
+  eapply weakening.
+  discriminate.
+Qed.
+
+Lemma substitution_preserves_typing : forall Gamma x U t v T,
+  x |-> U ; Gamma |- t \in T ->
+  empty |- v \in U   ->
+  Gamma |- [x:=v]t \in T.
+
+(** The substitution lemma can be viewed as a kind of "commutation
+    property."  Intuitively, it says that substitution and typing can
+    be done in either order: we can either assign types to the terms
+    [t] and [v] separately (under suitable contexts) and then combine
+    them using substitution, or we can substitute first and then
+    assign a type to [ [x:=v] t ]; the result is the same either
+    way.
+
+    _Proof_: We show, by induction on [t], that for all [T] and
+    [Gamma], if [x|->U; Gamma |- t \in T] and [|- v \in U], then
+    [Gamma |- [x:=v]t \in T].
+
+      - If [t] is a variable there are two cases to consider,
+        depending on whether [t] is [x] or some other variable.
+
+          - If [t = x], then from the fact that [x|->U; Gamma |- x \in
+            T] we conclude that [U = T].  We must show that [[x:=v]x =
+            v] has type [T] under [Gamma], given the assumption that
+            [v] has type [U = T] under the empty context.  This
+            follows from the weakening lemma.
+
+          - If [t] is some variable [y] that is not equal to [x], then
+            we need only note that [y] has the same type under [x|->U;
+            Gamma] as under [Gamma].
+
+      - If [t] is an abstraction [\y:S, t0], then [T = S->T1] and
+        the IH tells us, for all [Gamma'] and [T0], that if [x|->U;
+        Gamma' |- t0 \in T0], then [Gamma' |- [x:=v]t0 \in T0].
+        Moreover, by inspecting the typing rules we see it must be
+        the case that [y|->S; x|->U; Gamma |- t0 \in T1].
+
+        The substitution in the conclusion behaves differently
+        depending on whether [x] and [y] are the same variable.
+
+        First, suppose [x = y].  Then, by the definition of
+        substitution, [[x:=v]t = t], so we just need to show [Gamma |-
+        t \in T].  Using [T_Abs], we need to show that [y|->S; Gamma
+        |- t0 \in T1]. But we know [y|->S; x|->U; Gamma |- t0 \in T1],
+        and the claim follows since [x = y].
+
+        Second, suppose [x <> y]. Again, using [T_Abs],
+        we need to show that [y|->S; Gamma |- [x:=v]t0 \in T1].
+        Since [x <> y], we have
+        [y|->S; x|->U; Gamma = x|->U; y|->S; Gamma]. So,
+        we have [x|->U; y|->S; Gamma |- t0 \in T1]. Then, the
+        the IH applies (taking [Gamma' = y|->S; Gamma]), giving us
+        [y|->S; Gamma |- [x:=v]t0 \in T1], as required.
+
+      - If [t] is an application [t1 t2], the result follows
+        straightforwardly from the definition of substitution and the
+        induction hypotheses.
+
+      - The remaining cases are similar to the application case. *)
+
+Proof.
+  intros Gamma x U t v T Ht Hv.
+  generalize dependent Gamma. generalize dependent T.
+  induction t; intros T Gamma H;
+  (* in each case, we'll want to get at the derivation of H *)
+    inversion H; clear H; subst; simpl; eauto.
+  - (* var *)
+    rename s into y. destruct (eqb_stringP x y); subst.
+    + (* x=y *)
+      rewrite update_eq in H2.
+      injection H2 as H2; subst.
+      apply weakening_empty. assumption.
+    + (* x<>y *)
+      apply T_Var. rewrite update_neq in H2; auto.
+  - (* abs *)
+    rename s into y, t into S.
+    destruct (eqb_stringP x y); subst; apply T_Abs.
+    + (* x=y *)
+      rewrite update_shadow in H5. assumption.
+    + (* x<>y *)
+      apply IHt.
+      rewrite update_permute; auto.
+Qed.
+
+Theorem preservation : forall t t' T,
+  empty |- t \in T  ->
+  t --> t'  ->
+  empty |- t' \in T.
+
+(** _Proof_: By induction on the derivation of [|- t \in T].
+
+    - We can immediately rule out [T_Var], [T_Abs], [T_Const], [T_Succ],
+     or [T_Mult] as final rules in the derivation, since in each of these
+     cases [t] cannot take a step.
+
+    - If the last rule in the derivation is [T_App], then [t = t1 t2],
+      and there are subderivations showing that [|- t1 \in T2->T] and
+      [|- t2 \in T2] plus two induction hypotheses: (1) [t1 --> t1']
+      implies [|- t1' \in T2->T] and (2) [t2 --> t2'] implies [|- t2'
+      \in T2].  There are now three subcases to consider, one for
+      each rule that could be used to show that [t1 t2] takes a step
+      to [t'].
+
+        - If [t1 t2] takes a step by [ST_App1], with [t1] stepping to
+          [t1'], then, by the first IH, [t1'] has the same type as
+          [t1] ([|- t1' \in T2->T]), and hence by [T_App] [t1' t2] has
+          type [T].
+
+        - The [ST_App2] case is similar, using the second IH.
+
+        - If [t1 t2] takes a step by [ST_AppAbs], then [t1 =
+          \x:T0,t0] and [t1 t2] steps to [[x0:=t2]t0]; the desired
+          result now follows from the substitution lemma.
+
+    - If the last rule in the derivation is [T_If0], then [t = if0
+      t1 then t2 else t3], with [|- t1 \in Nat], [|- t2 \in T1], and
+      [|- t3 \in T1], and with three induction hypotheses: (1) [t1 -->
+      t1'] implies [|- t1' \in Nat], (2) [t2 --> t2'] implies [|- t2'
+      \in T1], and (3) [t3 --> t3'] implies [|- t3' \in T1].
+
+      There are again three subcases to consider, depending on how [t]
+      steps.
+
+        - If [t] steps to [t2] or [t3] by [ST_If0Zero] or
+          [ST_If0Succ], the result is immediate, since [t2] and [t3]
+          have the same type as [t].
+
+        - Otherwise, [t] steps by [ST_If0], and the desired
+          conclusion follows directly from the first induction
+          hypothesis. 
+
+    - If the last rule in the derivation is [T_Pred], then [t = pred t1],
+      with [|- t1 \in Nat]. and with the induction hypothesis:
+      [t1 --> t1'] implies [|- t1' \in Nat]. There are three subcases to
+      consider, depending on how [t] steps.
+
+        - If [t1] is a const value [n], then [t --> tm_const (pred n)] by
+          [ST_PredNat]. It is immediate that [|- (pred n) \in Nat].
+
+        - If [t1 --> t1'], then [t --> pred t1'] by [ST_Pred]. From the
+          induction hypothesis with [T_Pred], it is immediate
+          that [|- pred t1' \in Nat].
+
+        - If [t1 = succ t1'], then [t --> t1'] by [ST_PredSucc]. 
+          Inversing the [T_Succ] we know immediately that [|- t1' \in Nat].
+*)
+
+Proof with eauto.
+  intros t t' T HT. generalize dependent t'.
+  remember empty as Gamma.
+  induction HT;
+       intros t' HE; subst;
+       try solve [inversion HE; subst; auto].
+  - (* T_App *)
+    inversion HE; subst...
+    (* Most of the cases are immediate by induction,
+       and [eauto] takes care of them *)
+    + (* ST_AppAbs *)
+      apply substitution_preserves_typing with T2...
+      inversion HT1...
+  - (* T_Pred *)
+    inversion HE; subst...
+    (* Most of the cases are immediate by inducition,
+      and [eauto] takes care of them *)
+    + (* ST_PredSucc *)
+      inversion HT; subst...
+Qed.
+
+Lemma canonical_forms_nat : forall t,
+  empty |- t \in Nat ->
+  value t ->
+  (exists n, t = tm_const n).
+Proof.
+  intros t HT HVal.
+  destruct HVal; auto.
+  inversion HT.
+  exists n; auto.
+Qed.
+
+Lemma canonical_forms_fun : forall t T1 T2,
+  empty |- t \in (T1 -> T2) ->
+  value t ->
+  exists x u, t = <{\x:T1, u}>.
+Proof.
+  intros t T1 T2 HT HVal.
+  destruct HVal; inversion HT; subst.
+  exists x0, t1. reflexivity.
+Qed.
+
+Theorem progress : forall t T,
+  empty |- t \in T ->
+  value t \/ exists t', t --> t'.
+
+(** _Proof_: By induction on the derivation of [|- t \in T].
+
+    - The last rule of the derivation cannot be [T_Var], since a
+      variable is never well typed in an empty context.
+
+    - The [T_Const], and [T_Abs] cases are trivial, since in
+      each of these cases we can see by inspecting the rule that [t]
+      is a value.
+
+    - If the last rule of the derivation is [T_App], then [t] has the
+      form [t1 t2] for some [t1] and [t2], where [|- t1 \in T2 -> T]
+      and [|- t2 \in T2] for some type [T2].  The induction hypothesis
+      for the first subderivation says that either [t1] is a value or
+      else it can take a reduction step.
+
+        - If [t1] is a value, then consider [t2], which by the
+          induction hypothesis for the second subderivation must also
+          either be a value or take a step.
+
+            - Suppose [t2] is a value.  Since [t1] is a value with an
+              arrow type, it must be a lambda abstraction; hence [t1
+              t2] can take a step by [ST_AppAbs].
+
+            - Otherwise, [t2] can take a step, and hence so can [t1
+              t2] by [ST_App2].
+
+        - If [t1] can take a step, then so can [t1 t2] by [ST_App1].
+
+    - If the last rule of the derivation is [T_Succ], then [t = succ 
+      t1], where [|- t1 \in Nat]. The induction hypothesis for [t1] 
+      says that either [t1] is a value or else it can take a reduction
+      step.
+
+        - If [t1] is a value, then by [canonical_forms_nat] we know
+          that [t1 = tm_const n], hence [succ t1] can take a step by
+          [ST_SuccNat].
+
+        - Otherwise, [t1] can take a step, and hence so can [succ t1]
+          by [ST_Succ].
+
+    - If the last rule of the derivation is [T_Pred], it is similar
+      with [T_Succ].
+
+    - If the last rule of the derivation is [T_Mult], then [t = t1 * 
+      t2], where [|- t1 \in Nat] and [|- t2 \in Nat]. The induction
+      hypothesis for [t1] and [t2] says each of them is either a value
+      or else it can take a reduction step.
+
+        - If [t1] and [t2] are both values, than by [canonical_forms_nat]
+          we knwo that [t1 = tm_const n1] and [t2 = tm_const n2], hence
+          [t1 * t2] can take a step by [ST_MultNat].
+
+        - If [t1] is a value and [t2] can take a step, and hence
+          [t1 * t2] can take a step by [ST_Mult2].
+
+        - If [t1] can take a step, and hence [t1 * t2] can take a step 
+          by [ST_Mult1].
+
+    - If the last rule of the derivation is [T_If0], then [t = if0
+      t1 then t2 else t3], where [t1] has type [Nat].  The first IH
+      says that [t1] either is a value or takes a step.
+
+        - If [t1] is a value, then since it has type [Nat] it must be
+          any const [n].  If it is [0], then [t] steps to [t2];
+          otherwise it steps to [t3].
+
+        - Otherwise, [t1] takes a step, and therefore so does [t] (by
+          [ST_If0]). *)
+Proof with eauto.
+  intros t T Ht.
+  remember empty as Gamma.
+  induction Ht; subst Gamma; auto.
+  (* auto solves all three cases in which t is a value *)
+  - (* T_Var *)
+    (* contradictory: variables cannot be typed in an
+       empty context *)
+    discriminate H.
+
+  - (* T_App *)
+    (* [t] = [t1 t2].  Proceed by cases on whether [t1] is a
+       value or steps... *)
+    right. destruct IHHt1...
+    + (* t1 is a value *)
+      destruct IHHt2...
+      * (* t2 is also a value *)
+        eapply canonical_forms_fun in Ht1; [|assumption].
+        destruct Ht1 as [x [t0 H1]]. subst.
+        exists (<{ [x:=t2]t0 }>)...
+      * (* t2 steps *)
+        destruct H0 as [t2' Hstp]. exists (<{t1 t2'}>)...
+
+    + (* t1 steps *)
+      destruct H as [t1' Hstp]. exists (<{t1' t2}>)...
+
+  - (* T_Succ *)
+    right. destruct IHHt...
+    + eapply canonical_forms_nat in Ht; [|assumption].
+      destruct Ht as [n Ht]. subst.
+      exists (S n)...
+    + destruct H as [t' H].  exists (<{succ t'}>)...
+
+  - (* T_Pred *)
+    right. destruct IHHt...
+    + eapply canonical_forms_nat in Ht; [|assumption].
+      destruct Ht as [n Ht]. subst.
+      exists (pred n)...
+    + destruct H as [t' H].  exists (<{pred t'}>)...
+
+  - (* T_Mult *)
+    right. destruct IHHt1...
+    + destruct IHHt2...
+      * eapply canonical_forms_nat in Ht1; [|assumption].
+        eapply canonical_forms_nat in Ht2; [|assumption].
+        destruct Ht1 as [n1 Ht1]; subst.
+        destruct Ht2 as [n2 Ht2]; subst.
+        exists (n1 * n2)...
+      * destruct H0 as [t2' H2]. exists (<{t1 * t2'}>)...
+    + destruct H as [t1' H]. exists (<{t1' * t2}>)...
+
+  - (* T_If0 *)
+    right. destruct IHHt1...
+
+    + (* t1 is a value *)
+      eapply canonical_forms_nat in H; [|assumption].
+      destruct H as [n H]; subst.
+      destruct n; eauto.
+
+    + (* t1 also steps *)
+      destruct H as [t1' Hstp]. exists <{if0 t1' then t2 else t3}>...
+Qed.
+
 
 (* Do not modify the following line: *)
 Definition manual_grade_for_stlc_arith : option (nat*string) := None.
